Ch3 scraps

Ch3.thy
@@ -2,4 +2,56 @@ theory Ch3
   imports Main
 begin
 
+type_synonym vname = string
+datatype aexp = N int | V vname | Plus aexp aexp
+type_synonym val = int
+type_synonym state = "vname \<Rightarrow> val"
+
+fun aval :: "aexp \<Rightarrow> state \<Rightarrow> val" where
+"aval (N n) s = n" |
+"aval (V x ) s = s x" |
+"aval (Plus a1 a2) s = aval a1 s + aval a2 s"
+
+(* 3.10 *)
+
+datatype instr = LOADI val | LOAD vname | ADD
+
+type_synonym stack = "val list"
+
+abbreviation hd2 where
+"hd2 xs \<equiv> hd (tl xs)"
+
+abbreviation tl2 where
+"tl2 xs \<equiv> tl (tl xs)"
+
+fun exec1 :: "instr \<Rightarrow> state \<Rightarrow> stack \<Rightarrow> stack option" where
+"exec1 (LOADI n) _ stk = Some (n # stk)" |
+"exec1 (LOAD x) s stk = Some (s(x) # stk)" |
+"exec1 ADD _ stk =
+ (case stk of
+  (x # y # xs) \<Rightarrow> Some ((hd2 stk + hd stk) # tl2 stk) |
+  (xs) \<Rightarrow> None)"
+
+fun exec :: "instr list \<Rightarrow> state \<Rightarrow> stack \<Rightarrow> stack option" where
+"exec [] _ stk = Some stk" |
+"exec (i#is) s stk =
+ (case (exec1 i s stk) of
+  Some res \<Rightarrow> exec is s res |
+  None \<Rightarrow> None)"
+
+fun comp :: "aexp \<Rightarrow> instr list" where
+"comp (N n) = [LOADI n]" |
+"comp (V x) = [LOAD x]" |
+"comp (Plus e1 e2) = comp e1 @ comp e2 @ [ADD]"
+
+lemma exec_append: "exec is1 s stk = Some new_stk \<Longrightarrow> exec (is1 @ is2) s stk = exec is2 s new_stk"
+apply (induction is1 arbitrary:stk)
+apply (auto split:option.split)
+done
+
+lemma "exec (comp a) s stk = Some (aval a s # stk)"
+apply (induction a arbitrary:stk)
+apply (auto simp add: exec_append)
+done
+
 end
